providers/evercrypt/fst/EverCrypt.CTR.Keys.fst
@@ -1,0 +1,5 @@
+module EverCrypt.CTR.Keys
+
+/// This is an internal-to-EverCrypt module, which provides low-level
+/// definitions corresponding to Spec.Cipher.Expansion, i.e. shared between CTR
+/// and AEAD.
